add transpose4x4 and transpose8x8 for t = U64

lib/Lib.IntVector.Transpose.fst
@@ -10,9 +10,8 @@ module Loops = Lib.LoopCombinators
 ///
 
 inline_for_extraction noextract
-val transpose4x4_uint32: #t:v_inttype{t == U32} -> vec_t4 t -> vec_t4 t
-let transpose4x4_uint32 #t vs =
-  let (v0,v1,v2,v3) = vs in
+val transpose4x4_0: #t:v_inttype -> vec_t4 t -> vec_t4 t
+let transpose4x4_0 #t (v0,v1,v2,v3) =
   let v0' = vec_interleave_low v0 v1 in
   let v1' = vec_interleave_high v0 v1 in
   let v2' = vec_interleave_low v2 v3 in
@@ -22,12 +21,26 @@ let transpose4x4_uint32 #t vs =
   let v1'' = vec_interleave_high_n 2 v0' v2' in
   let v2'' = vec_interleave_low_n 2 v1' v3' in
   let v3'' = vec_interleave_high_n 2 v1' v3' in
+  (v0'',v2'',v1'',v3'')
+
+
+inline_for_extraction noextract
+val transpose4x4_uint32: #t:v_inttype{t == U32} -> vec_t4 t -> vec_t4 t
+let transpose4x4_uint32 #t vs =
+  [@inline_let]
+  let (v0'',v2'',v1'',v3'') = transpose4x4_0 #t vs in
   (v0'',v1'',v2'',v3'')
+
+
+inline_for_extraction noextract
+val transpose4x4_uint64: #t:v_inttype{t == U64} -> vec_t4 t -> vec_t4 t
+let transpose4x4_uint64 #t vs = transpose4x4_0 #t vs
 
 
 let transpose4x4 #t vs =
   match t with
   | U32 -> transpose4x4_uint32 #t vs
+  | U64 -> transpose4x4_uint64 #t vs
   | _ -> admit()
 
 ///
@@ -35,8 +48,8 @@ let transpose4x4 #t vs =
 ///
 
 inline_for_extraction noextract
-val transpose8x8_uint32_0: #t:v_inttype{t == U32} -> vec_t8 t -> vec_t8 t
-let transpose8x8_uint32_0 #t (v0,v1,v2,v3,v4,v5,v6,v7) =
+val transpose8x8_0: #t:v_inttype -> vec_t8 t -> vec_t8 t
+let transpose8x8_0 #t (v0,v1,v2,v3,v4,v5,v6,v7) =
   let v0' = vec_interleave_low v0 v1 in
   let v1' = vec_interleave_high v0 v1 in
   let v2' = vec_interleave_low v2 v3 in
@@ -49,8 +62,8 @@ let transpose8x8_uint32_0 #t (v0,v1,v2,v3,v4,v5,v6,v7) =
 
 
 inline_for_extraction noextract
-val transpose8x8_uint32_1: #t:v_inttype{t == U32} -> vec_t8 t -> vec_t8 t
-let transpose8x8_uint32_1 #t (v0,v1,v2,v3,v4,v5,v6,v7) =
+val transpose8x8_1: #t:v_inttype -> vec_t8 t -> vec_t8 t
+let transpose8x8_1 #t (v0,v1,v2,v3,v4,v5,v6,v7) =
   let v0' = vec_interleave_low_n 2 v0 v2 in
   let v2' = vec_interleave_high_n 2 v0 v2 in
   let v1' = vec_interleave_low_n 2 v1 v3 in
@@ -63,8 +76,8 @@ let transpose8x8_uint32_1 #t (v0,v1,v2,v3,v4,v5,v6,v7) =
 
 
 inline_for_extraction noextract
-val transpose8x8_uint32_2: #t:v_inttype{t == U32} -> vec_t8 t -> vec_t8 t
-let transpose8x8_uint32_2 #t (v0,v1,v2,v3,v4,v5,v6,v7) =
+val transpose8x8_2: #t:v_inttype -> vec_t8 t -> vec_t8 t
+let transpose8x8_2 #t (v0,v1,v2,v3,v4,v5,v6,v7) =
   let v0' = vec_interleave_low_n 4 v0 v4 in
   let v4' = vec_interleave_high_n 4 v0 v4 in
   let v1' = vec_interleave_low_n 4 v1 v5 in
@@ -77,20 +90,36 @@ let transpose8x8_uint32_2 #t (v0,v1,v2,v3,v4,v5,v6,v7) =
 
 
 inline_for_extraction noextract
-val transpose8x8_uint32: #t:v_inttype{t == U32} -> vec_t8 t -> vec_t8 t
-let transpose8x8_uint32 #t vs0 =
+val transpose8x8_012: #t:v_inttype -> vec_t8 t -> vec_t8 t
+let transpose8x8_012 #t vs0 =
   let (v0,v1,v2,v3,v4,v5,v6,v7) = vs0 in
   [@inline_let]
-  let (v0',v1',v2',v3',v4',v5',v6',v7') = transpose8x8_uint32_0 #t (v0,v1,v2,v3,v4,v5,v6,v7) in
+  let (v0',v1',v2',v3',v4',v5',v6',v7') = transpose8x8_0 #t (v0,v1,v2,v3,v4,v5,v6,v7) in
   [@inline_let]
-  let (v0',v1',v2',v3',v4',v5',v6',v7') = transpose8x8_uint32_1 #t (v0',v1',v2',v3',v4',v5',v6',v7') in
+  let (v0',v1',v2',v3',v4',v5',v6',v7') = transpose8x8_1 #t (v0',v1',v2',v3',v4',v5',v6',v7') in
   [@inline_let]
-  let (v0',v1',v2',v3',v4',v5',v6',v7') = transpose8x8_uint32_2 #t (v0',v1',v2',v3',v4',v5',v6',v7') in
+  let (v0',v1',v2',v3',v4',v5',v6',v7') = transpose8x8_2 #t (v0',v1',v2',v3',v4',v5',v6',v7') in
+  (v0',v1',v2',v3',v4',v5',v6',v7')
+
+
+inline_for_extraction noextract
+val transpose8x8_uint32: #t:v_inttype{t == U32} -> vec_t8 t -> vec_t8 t
+let transpose8x8_uint32 #t vs0 =
+  [@inline_let]
+  let (v0',v1',v2',v3',v4',v5',v6',v7') = transpose8x8_012 #t vs0 in
   (v0',v2',v1',v3',v4',v6',v5',v7')
+
+
+inline_for_extraction noextract
+val transpose8x8_uint64: #t:v_inttype{t == U64} -> vec_t8 t -> vec_t8 t
+let transpose8x8_uint64 #t vs0 =
+  transpose8x8_012 #t vs0
+
 
 let transpose8x8 #t vs =
   match t with
   | U32 -> transpose8x8_uint32 #t vs
+  | U64 -> transpose8x8_uint64 #t vs
   | _ -> admit()
 
 ///
@@ -255,15 +284,16 @@ let lemma_l_plus_pow2i_lt #w n i l =
 
 
 inline_for_extraction noextract
-val transposewxw_uint32_f_l:
+val transposewxw_f_l:
     #w:width
+  -> #t:v_inttype
   -> n:nat{pow2 n == w}
   -> i:nat{i < n}
-  -> lseq (vec_t U32 w) w
+  -> lseq (vec_t t w) w
   -> l:nat{l < w} ->
-  vec_t U32 w
+  vec_t t w
 
-let transposewxw_uint32_f_l #w n i vs l =
+let transposewxw_f_l #w #t n i vs l =
   Math.Lemmas.pow2_multiplication_modulo_lemma_1 1 i n;
   if l % (2 * pow2 i) < pow2 i
   then begin
@@ -274,27 +304,33 @@ let transposewxw_uint32_f_l #w n i vs l =
 
 
 inline_for_extraction noextract
-val transposewxw_uint32_f: #w:width -> n:nat{pow2 n == w} -> i:nat{i < n} -> lseq (vec_t U32 w) w -> lseq (vec_t U32 w) w
-let transposewxw_uint32_f #w n i vs =
-  createi w (transposewxw_uint32_f_l #w n i vs)
+val transposewxw_f: #w:width -> #t:v_inttype -> n:nat{pow2 n == w} -> i:nat{i < n} -> lseq (vec_t t w) w -> lseq (vec_t t w) w
+let transposewxw_f #w #t n i vs =
+  createi w (transposewxw_f_l #w n i vs)
 
-val transposewxw_uint32_lseq: #w:width -> n:nat{pow2 n == w} -> vs:lseq (vec_t U32 w) w -> lseq (vec_t U32 w) w
-let transposewxw_uint32_lseq #w n vs =
-  Loops.repeati n (transposewxw_uint32_f #w n) vs
+val transposewxw_lseq: #w:width -> #t:v_inttype -> n:nat{pow2 n == w} -> vs:lseq (vec_t t w) w -> lseq (vec_t t w) w
+let transposewxw_lseq #w #t n vs =
+  Loops.repeati n (transposewxw_f #w n) vs
 
 ///
 ///  transposewxw_lseq lemmas
 ///
-val transpose4x4_lseq_is_transposewxw_uint32: vs:lseq (vec_t U32 4) 4 ->
-  Lemma
-   (let r = transposewxw_uint32_lseq 2 vs in
-    create4 r.[0] r.[2] r.[1] r.[3] `Seq.equal` transpose4x4_lseq #U32 vs)
 
-let transpose4x4_lseq_is_transposewxw_uint32 vs0 =
+inline_for_extraction noextract
+let f_lseq4 (#t:v_inttype) (vs:lseq (vec_t t 4) 4) (f:vec_t4 t -> vec_t4 t) : lseq (vec_t t 4) 4 =
+  let (v0,v1,v2,v3) = (vs.[0],vs.[1],vs.[2],vs.[3]) in
+  let (r0,r1,r2,r3) = f (v0,v1,v2,v3) in
+  create4 r0 r1 r2 r3
+
+val transpose4x4_lseq_is_transposewxw: #t:v_inttype -> vs:lseq (vec_t t 4) 4 ->
+  Lemma (transposewxw_lseq 2 vs `Seq.equal` f_lseq4 vs transpose4x4_0)
+
+let transpose4x4_lseq_is_transposewxw #t vs0 =
   let n = 2 in
-  Loops.unfold_repeati n (transposewxw_uint32_f #4 n) vs0 1;
-  Loops.unfold_repeati n (transposewxw_uint32_f #4 n) vs0 0;
-  Loops.eq_repeati0 n (transposewxw_uint32_f #4 n) vs0
+  Loops.unfold_repeati n (transposewxw_f #4 n) vs0 1;
+  Loops.unfold_repeati n (transposewxw_f #4 n) vs0 0;
+  Loops.eq_repeati0 n (transposewxw_f #4 n) vs0;
+  eq_intro (transposewxw_lseq 2 vs0) (f_lseq4 vs0 transpose4x4_0)
 
 
 inline_for_extraction noextract
@@ -304,27 +340,23 @@ let f_lseq8 (#t:v_inttype) (vs:lseq (vec_t t 8) 8) (f:vec_t8 t -> vec_t8 t) : ls
   create8 r0 r1 r2 r3 r4 r5 r6 r7
 
 
-val transpose8x8_lseq_is_transposewxw_uint32: vs:lseq (vec_t U32 8) 8 ->
-  Lemma
-   (let r = transposewxw_uint32_lseq 3 vs in
-    create8 r.[0] r.[2] r.[1] r.[3] r.[4] r.[6] r.[5] r.[7] `Seq.equal` transpose8x8_lseq #U32 vs)
+val transpose8x8_lseq_is_transposewxw: #t:v_inttype -> vs:lseq (vec_t t 8) 8 ->
+  Lemma (transposewxw_lseq 3 vs `Seq.equal` f_lseq8 vs transpose8x8_012)
 
-let transpose8x8_lseq_is_transposewxw_uint32 vs0 =
+let transpose8x8_lseq_is_transposewxw #t vs0 =
   let n = 3 in
-  Loops.unfold_repeati n (transposewxw_uint32_f #8 n) vs0 2;
-  Loops.unfold_repeati n (transposewxw_uint32_f #8 n) vs0 1;
-  Loops.unfold_repeati n (transposewxw_uint32_f #8 n) vs0 0;
-  Loops.eq_repeati0 n (transposewxw_uint32_f #8 n) vs0;
-  let r = transposewxw_uint32_lseq 3 vs0 in
-  let res = create8 r.[0] r.[2] r.[1] r.[3] r.[4] r.[6] r.[5] r.[7] in
+  Loops.unfold_repeati n (transposewxw_f #8 n) vs0 2;
+  Loops.unfold_repeati n (transposewxw_f #8 n) vs0 1;
+  Loops.unfold_repeati n (transposewxw_f #8 n) vs0 0;
+  Loops.eq_repeati0 n (transposewxw_f #8 n) vs0;
 
-  let res0 = transposewxw_uint32_f n 0 vs0 in
-  eq_intro res0 (f_lseq8 vs0 transpose8x8_uint32_0);
-  let res1 = transposewxw_uint32_f n 1 res0 in
-  eq_intro res1 (f_lseq8 res0 transpose8x8_uint32_1);
-  let res2 = transposewxw_uint32_f n 2 res1 in
-  eq_intro res2 (f_lseq8 res1 transpose8x8_uint32_2);
-  eq_intro res (f_lseq8 vs0 transpose8x8)
+  let res0 = transposewxw_f n 0 vs0 in
+  eq_intro res0 (f_lseq8 vs0 transpose8x8_0);
+  let res1 = transposewxw_f n 1 res0 in
+  eq_intro res1 (f_lseq8 res0 transpose8x8_1);
+  let res2 = transposewxw_f n 2 res1 in
+  eq_intro res2 (f_lseq8 res1 transpose8x8_2);
+  eq_intro (transposewxw_lseq 3 vs0) (f_lseq8 vs0 transpose8x8_012)
 
 
 inline_for_extraction noextract
@@ -337,47 +369,49 @@ let f_lseq16 (#t:v_inttype) (vs:lseq (vec_t t 16) 16)
     f ((v0,v1,v2,v3,v4,v5,v6,v7), (v8,v9,v10,v11,v12,v13,v14,v15)) in
   create16 r0 r1 r2 r3 r4 r5 r6 r7 r8 r9 r10 r11 r12 r13 r14 r15
 
+
 #push-options "--z3rlimit 100"
 val transpose16x16_lseq_is_transposewxw_uint32: vs:lseq (vec_t U32 16) 16 ->
   Lemma
-   (let r = transposewxw_uint32_lseq 4 vs in
+   (let r = transposewxw_lseq 4 vs in
     create16 r.[0] r.[2] r.[1] r.[3] r.[4] r.[6] r.[5] r.[7] r.[8] r.[10] r.[9] r.[11] r.[12] r.[14] r.[13] r.[15]
       `Seq.equal` transpose16x16_lseq #U32 vs)
 
 let transpose16x16_lseq_is_transposewxw_uint32 vs0 =
   let n = 4 in
-  Loops.unfold_repeati n (transposewxw_uint32_f #16 n) vs0 3;
-  Loops.unfold_repeati n (transposewxw_uint32_f #16 n) vs0 2;
-  Loops.unfold_repeati n (transposewxw_uint32_f #16 n) vs0 1;
-  Loops.unfold_repeati n (transposewxw_uint32_f #16 n) vs0 0;
-  Loops.eq_repeati0 n (transposewxw_uint32_f #16 n) vs0;
-  let r = transposewxw_uint32_lseq n vs0 in
+  Loops.unfold_repeati n (transposewxw_f #16 n) vs0 3;
+  Loops.unfold_repeati n (transposewxw_f #16 n) vs0 2;
+  Loops.unfold_repeati n (transposewxw_f #16 n) vs0 1;
+  Loops.unfold_repeati n (transposewxw_f #16 n) vs0 0;
+  Loops.eq_repeati0 n (transposewxw_f #16 n) vs0;
+  let r = transposewxw_lseq n vs0 in
 
-  let res0 = transposewxw_uint32_f n 0 vs0 in
+  let res0 = transposewxw_f n 0 vs0 in
   eq_intro res0 (f_lseq16 vs0 transpose16x16_uint32_0);
-  let res1 = transposewxw_uint32_f n 1 res0 in
+  let res1 = transposewxw_f n 1 res0 in
   eq_intro res1 (f_lseq16 res0 transpose16x16_uint32_1);
-  let res2 = transposewxw_uint32_f n 2 res1 in
+  let res2 = transposewxw_f n 2 res1 in
   eq_intro res2 (f_lseq16 res1 transpose16x16_uint32_2);
-  let res3 = transposewxw_uint32_f n 3 res2 in
+  let res3 = transposewxw_f n 3 res2 in
   eq_intro res3 (f_lseq16 res2 transpose16x16_uint32_3);
   let res = create16 r.[0] r.[2] r.[1] r.[3] r.[4] r.[6] r.[5] r.[7] r.[8] r.[10] r.[9] r.[11] r.[12] r.[14] r.[13] r.[15] in
   eq_intro res (f_lseq16 vs0 transpose16x16_uint32)
 #pop-options
 
-val transpose4x4_lemma_ij: vs:lseq (vec_t U32 4) 4 -> i:nat{i < 4} -> j:nat{j < 4} ->
+
+val transpose4x4_lemma_uint32_ij: vs:lseq (vec_t U32 4) 4 -> i:nat{i < 4} -> j:nat{j < 4} ->
   Lemma ((vec_v (transpose4x4_lseq #U32 vs).[i]).[j] == (vec_v vs.[j]).[i])
 
-let transpose4x4_lemma_ij vs0 i j =
-  transpose4x4_lseq_is_transposewxw_uint32 vs0;
+let transpose4x4_lemma_uint32_ij vs0 i j =
+  transpose4x4_lseq_is_transposewxw vs0;
   let n = 2 in
-  let r = transposewxw_uint32_lseq 2 vs0 in
-  Loops.unfold_repeati n (transposewxw_uint32_f #4 n) vs0 1;
-  Loops.unfold_repeati n (transposewxw_uint32_f #4 n) vs0 0;
-  Loops.eq_repeati0 n (transposewxw_uint32_f #4 n) vs0;
+  let r = transposewxw_lseq 2 vs0 in
+  Loops.unfold_repeati n (transposewxw_f #4 n) vs0 1;
+  Loops.unfold_repeati n (transposewxw_f #4 n) vs0 0;
+  Loops.eq_repeati0 n (transposewxw_f #4 n) vs0;
 
-  let res0 = transposewxw_uint32_f 2 0 vs0 in
-  let res1 = transposewxw_uint32_f 2 1 res0 in
+  let res0 = transposewxw_f 2 0 vs0 in
+  let res1 = transposewxw_f 2 1 res0 in
 
   vec_interleave_low_n_lemma_uint32_4_2 res0.[0] res0.[2];
   vec_interleave_high_n_lemma_uint32_4_2 res0.[0] res0.[2];
@@ -390,20 +424,45 @@ let transpose4x4_lemma_ij vs0 i j =
   vec_interleave_high_lemma_uint32_4 vs0.[2] vs0.[3]
 
 
-val transpose8x8_lemma_ij: vs:lseq (vec_t U32 8) 8 -> i:nat{i < 8} -> j:nat{j < 8} ->
+val transpose4x4_lemma_uint64_ij: vs:lseq (vec_t U64 4) 4 -> i:nat{i < 4} -> j:nat{j < 4} ->
+  Lemma ((vec_v (transpose4x4_lseq #U64 vs).[i]).[j] == (vec_v vs.[j]).[i])
+
+let transpose4x4_lemma_uint64_ij vs0 i j =
+  transpose4x4_lseq_is_transposewxw vs0;
+  let n = 2 in
+  let r = transposewxw_lseq 2 vs0 in
+  Loops.unfold_repeati n (transposewxw_f #4 n) vs0 1;
+  Loops.unfold_repeati n (transposewxw_f #4 n) vs0 0;
+  Loops.eq_repeati0 n (transposewxw_f #4 n) vs0;
+
+  let res0 = transposewxw_f 2 0 vs0 in
+  let res1 = transposewxw_f 2 1 res0 in
+
+  vec_interleave_low_n_lemma_uint64_4_2 res0.[0] res0.[2];
+  vec_interleave_high_n_lemma_uint64_4_2 res0.[0] res0.[2];
+  vec_interleave_low_n_lemma_uint64_4_2 res0.[1] res0.[3];
+  vec_interleave_high_n_lemma_uint64_4_2 res0.[1] res0.[3];
+
+  vec_interleave_low_lemma_uint64_4 vs0.[0] vs0.[1];
+  vec_interleave_high_lemma_uint64_4 vs0.[0] vs0.[1];
+  vec_interleave_low_lemma_uint64_4 vs0.[2] vs0.[3];
+  vec_interleave_high_lemma_uint64_4 vs0.[2] vs0.[3]
+
+
+val transpose8x8_lemma_uint32_ij: vs:lseq (vec_t U32 8) 8 -> i:nat{i < 8} -> j:nat{j < 8} ->
   Lemma ((vec_v (transpose8x8_lseq #U32 vs).[i]).[j] == (vec_v vs.[j]).[i])
 
-let transpose8x8_lemma_ij vs0 i j =
-  transpose8x8_lseq_is_transposewxw_uint32 vs0;
+let transpose8x8_lemma_uint32_ij vs0 i j =
+  transpose8x8_lseq_is_transposewxw vs0;
   let n = 3 in
-  Loops.unfold_repeati n (transposewxw_uint32_f #8 n) vs0 2;
-  Loops.unfold_repeati n (transposewxw_uint32_f #8 n) vs0 1;
-  Loops.unfold_repeati n (transposewxw_uint32_f #8 n) vs0 0;
-  Loops.eq_repeati0 n (transposewxw_uint32_f #8 n) vs0;
+  Loops.unfold_repeati n (transposewxw_f #8 n) vs0 2;
+  Loops.unfold_repeati n (transposewxw_f #8 n) vs0 1;
+  Loops.unfold_repeati n (transposewxw_f #8 n) vs0 0;
+  Loops.eq_repeati0 n (transposewxw_f #8 n) vs0;
 
-  let res0 = transposewxw_uint32_f n 0 vs0 in
-  let res1 = transposewxw_uint32_f n 1 res0 in
-  let res2 = transposewxw_uint32_f n 2 res1 in
+  let res0 = transposewxw_f n 0 vs0 in
+  let res1 = transposewxw_f n 1 res0 in
+  let res2 = transposewxw_f n 2 res1 in
 
   vec_interleave_low_n_lemma_uint32_8_4 res1.[0] res1.[4];
   vec_interleave_low_n_lemma_uint32_8_4 res1.[1] res1.[5];
@@ -433,6 +492,49 @@ let transpose8x8_lemma_ij vs0 i j =
   vec_interleave_high_lemma_uint32_8 vs0.[6] vs0.[7]
 
 
+val transpose8x8_lemma_uint64_ij: vs:lseq (vec_t U64 8) 8 -> i:nat{i < 8} -> j:nat{j < 8} ->
+  Lemma ((vec_v (transpose8x8_lseq #U64 vs).[i]).[j] == (vec_v vs.[j]).[i])
+
+let transpose8x8_lemma_uint64_ij vs0 i j =
+  transpose8x8_lseq_is_transposewxw vs0;
+  let n = 3 in
+  Loops.unfold_repeati n (transposewxw_f #8 n) vs0 2;
+  Loops.unfold_repeati n (transposewxw_f #8 n) vs0 1;
+  Loops.unfold_repeati n (transposewxw_f #8 n) vs0 0;
+  Loops.eq_repeati0 n (transposewxw_f #8 n) vs0;
+
+  let res0 = transposewxw_f n 0 vs0 in
+  let res1 = transposewxw_f n 1 res0 in
+  let res2 = transposewxw_f n 2 res1 in
+
+  vec_interleave_low_n_lemma_uint64_8_4 res1.[0] res1.[4];
+  vec_interleave_low_n_lemma_uint64_8_4 res1.[1] res1.[5];
+  vec_interleave_low_n_lemma_uint64_8_4 res1.[2] res1.[6];
+  vec_interleave_low_n_lemma_uint64_8_4 res1.[3] res1.[7];
+  vec_interleave_high_n_lemma_uint64_8_4 res1.[0] res1.[4];
+  vec_interleave_high_n_lemma_uint64_8_4 res1.[1] res1.[5];
+  vec_interleave_high_n_lemma_uint64_8_4 res1.[2] res1.[6];
+  vec_interleave_high_n_lemma_uint64_8_4 res1.[3] res1.[7];
+
+  vec_interleave_low_n_lemma_uint64_8_2 res0.[0] res0.[2];
+  vec_interleave_low_n_lemma_uint64_8_2 res0.[1] res0.[3];
+  vec_interleave_low_n_lemma_uint64_8_2 res0.[4] res0.[6];
+  vec_interleave_low_n_lemma_uint64_8_2 res0.[5] res0.[7];
+  vec_interleave_high_n_lemma_uint64_8_2 res0.[0] res0.[2];
+  vec_interleave_high_n_lemma_uint64_8_2 res0.[1] res0.[3];
+  vec_interleave_high_n_lemma_uint64_8_2 res0.[4] res0.[6];
+  vec_interleave_high_n_lemma_uint64_8_2 res0.[5] res0.[7];
+
+  vec_interleave_low_lemma_uint64_8 vs0.[0] vs0.[1];
+  vec_interleave_low_lemma_uint64_8 vs0.[2] vs0.[3];
+  vec_interleave_low_lemma_uint64_8 vs0.[4] vs0.[5];
+  vec_interleave_low_lemma_uint64_8 vs0.[6] vs0.[7];
+  vec_interleave_high_lemma_uint64_8 vs0.[0] vs0.[1];
+  vec_interleave_high_lemma_uint64_8 vs0.[2] vs0.[3];
+  vec_interleave_high_lemma_uint64_8 vs0.[4] vs0.[5];
+  vec_interleave_high_lemma_uint64_8 vs0.[6] vs0.[7]
+
+
 #push-options "--z3rlimit 200"
 val transpose16x16_lemma_ij: vs:lseq (vec_t U32 16) 16 -> i:nat{i < 16} -> j:nat{j < 16} ->
   Lemma ((vec_v (transpose16x16_lseq #U32 vs).[i]).[j] == (vec_v vs.[j]).[i])
@@ -440,16 +542,16 @@ val transpose16x16_lemma_ij: vs:lseq (vec_t U32 16) 16 -> i:nat{i < 16} -> j:nat
 let transpose16x16_lemma_ij vs0 i j =
   transpose16x16_lseq_is_transposewxw_uint32 vs0;
 
-  Loops.unfold_repeati 4 (transposewxw_uint32_f 4) vs0 3;
-  Loops.unfold_repeati 4 (transposewxw_uint32_f 4) vs0 2;
-  Loops.unfold_repeati 4 (transposewxw_uint32_f 4) vs0 1;
-  Loops.unfold_repeati 4 (transposewxw_uint32_f 4) vs0 0;
-  Loops.eq_repeati0 4 (transposewxw_uint32_f 4) vs0;
+  Loops.unfold_repeati 4 (transposewxw_f 4) vs0 3;
+  Loops.unfold_repeati 4 (transposewxw_f 4) vs0 2;
+  Loops.unfold_repeati 4 (transposewxw_f 4) vs0 1;
+  Loops.unfold_repeati 4 (transposewxw_f 4) vs0 0;
+  Loops.eq_repeati0 4 (transposewxw_f 4) vs0;
 
-  let res0 = transposewxw_uint32_f 4 0 vs0 in
-  let res1 = transposewxw_uint32_f 4 1 res0 in
-  let res2 = transposewxw_uint32_f 4 2 res1 in
-  let res3 = transposewxw_uint32_f 4 3 res2 in
+  let res0 = transposewxw_f 4 0 vs0 in
+  let res1 = transposewxw_f 4 1 res0 in
+  let res2 = transposewxw_f 4 2 res1 in
+  let res3 = transposewxw_f 4 3 res2 in
 
   vec_interleave_low_n_lemma_uint32_16_8 res2.[0] res2.[8];
   vec_interleave_low_n_lemma_uint32_16_8 res2.[1] res2.[9];
@@ -527,13 +629,17 @@ let transpose16x16_lemma_ij vs0 i j =
 
 let transpose4x4_lemma #t vs =
   match t with
-  | U32 -> Classical.forall_intro_2 (transpose4x4_lemma_ij vs)
+  | U32 -> Classical.forall_intro_2 (transpose4x4_lemma_uint32_ij vs)
+  | U64 -> Classical.forall_intro_2 (transpose4x4_lemma_uint64_ij vs)
   | _ -> admit()
+
 
 let transpose8x8_lemma #t vs =
   match t with
-  | U32 -> Classical.forall_intro_2 (transpose8x8_lemma_ij vs)
+  | U32 -> Classical.forall_intro_2 (transpose8x8_lemma_uint32_ij vs)
+  | U64 -> Classical.forall_intro_2 (transpose8x8_lemma_uint64_ij vs)
   | _ -> admit()
+
 
 let transpose16x16_lemma #t vs =
   match t with
